icounter.fst
@@ -8,31 +8,51 @@ type o =
 
 type s = nat
 
-val apply_op : s -> o -> s
-let apply_op s (Inc n) = s + n
+val app_op : s -> o -> s
+let app_op s (Inc n) = s + n
 
-instance _ : datatype s o = {
-  History.apply_op = apply_op
+instance icounter : datatype s o = {
+  History.apply_op = app_op
 }
 
-val merge : {| datatype s o |}
-          -> h:history s o{wellformed h}
+val le : nat -> nat -> bool
+let le a b = a <= b
+
+val lemma1 : tr:list o -> s1:s
+           -> Lemma (ensures (le s1 (fold_left apply_op s1 tr)))
+let rec lemma1 tr s1 =
+  match tr with
+  | [] -> ()
+  | op::ops ->
+     let s2 = app_op s1 op in
+     lemma1 ops s2
+
+val merge : h:history s o{wellformed h}
           -> a:history s o{hbeq h a}
           -> b:history s o{hbeq h b}
-          -> l:history s o{forall h'. mem h' (lca h a b) ==> h' = l}
+          -> l:history s o{lca h a b = [l]}
           -> s
-let merge h a b l = admit ()
-  // get_state a + get_state b - get_state l
+let merge h a b l = 
+  History.lemma1 h;
+  assert (wellformed a);
+  assert (wellformed l);
 
-val commutativity : {| datatype s o |}
-                  -> h:history s o{wellformed h}
+  let tr = get_trace l a in
+  assert (fold_left apply_op (get_state l) tr = get_state a);
+
+  lemma1 tr (get_state l);
+  assert (get_state a >= get_state l);
+
+  get_state a + get_state b - get_state l
+
+val commutativity : h:history s o{wellformed h}
                   -> a:history s o{hbeq h a}
                   -> b:history s o{hbeq h b}
-                  -> l:history s o{forall h'. mem h' (lca h a b) ==> h' = l}
+                  -> l:history s o{lca h a b = [l] /\ lca h b a = [l]}
                   -> Lemma (ensures (merge h a b l = merge h b a l))
-let commutativity h a b l = admit ()
+let commutativity h a b l = ()
 
-instance _ : mrdt s o = {
+instance _ : mrdt s o icounter = {
   History.merge = merge;
   History.commutativity = commutativity
 }
